\documentclass[class=report, crop=false, 12pt,a4paper]{standalone}
\usepackage{enumitem}
\usepackage{multicol}
\usepackage{graphicx}
\usepackage{float}
\usepackage{amsmath}
\usepackage{amssymb}
\usepackage{mathtools}
\usepackage{siunitx}
\usepackage{commath}
\usepackage{array}
\usepackage{natbib}
\usepackage[a4paper,width=150mm,top=25mm,bottom=25mm]{geometry}
\setlength{\parindent}{0pt}
\begin{document}
\section{Statically Indeterminate Beams}
\begin{center}
  30/10/2020
\end{center}
So far, we have analysed statically-determinate beams. These are characterised by only \textbf{two unknown support reactions}, that can be determined from the force and moment equilibrium equations. \\\\
If the supports produce \textbf{three or more unknown reactions}, the beam is \textbf{statically indeterminate}.
\begin{figure}[H]
  \centering
  \includegraphics[width = 0.8 \textwidth]{../img/beam11.PNG}
\end{figure}
The analysis of statically indeterminate structures requires the calculation of displacements to find a sufficient number of equations to solve for all unknown reactions. \\\\
The double integration method or the Macaulayâ€™s method can be used to find the support reactions and the solution in statically indeterminate problems.
\subsubsection{Example: Propped Cantilever with Uniformly Distributed Load (Double Integration Method)}
\begin{figure}[H]
  \centering
  \includegraphics[width = 0.9 \textwidth]{../img/beam12.PNG}
\end{figure}
The equilibrium equations:
\begin{gather}
  R_A-wl+R_B = 0 \\
  R_Al-M_A-\frac{1}{2}wl^2 = 0
\end{gather}
Moment at the point distance $x$ away from the left end:
\begin{gather}
  M(x) = -M_A-\frac{1}{2}wx^2+R_Ax
\end{gather}
Integrating the moment equation:
\begin{gather}
  \theta(x) = \frac{\dif y}{\dif x} = -\frac{1}{EI}\int\left(-M_A-\frac{1}{2}wx^2+R_Ax\right)\dif x \\
  = -\frac{1}{EI}\left(-M_Ax-\frac{1}{6}wx^3+\frac{1}{2}R_Ax^2\right) + \theta_0
\end{gather}
Boundary Condition: $\theta(0) = 0 \longrightarrow \theta_0 = 0$
\begin{gather}
  \therefore \theta(x) = -\frac{1}{EI}\left(-M_Ax-\frac{1}{6}wx^3+\frac{1}{2}R_Ax^2\right)
\end{gather}
Integrating further:
\begin{gather}
  y(x) = -\frac{1}{EI}\int\left(-M_Ax-\frac{1}{6}wx^3+\frac{1}{2}R_Ax^2\right)\dif x \\
  = -\frac{1}{EI}\left(-\frac{1}{2}M_Ax^2-\frac{1}{24}wx^4+\frac{1}{6}R_Ax^3\right) + y_0
\end{gather}
Boundary Condition: $y(0) = 0 \longrightarrow y_0 = 0$
\begin{gather}
  \therefore y(x) = -\frac{1}{EI}\left(-\frac{1}{2}M_Ax^2-\frac{1}{24}wx^4+\frac{1}{6}R_Ax^3\right)
\end{gather}
Applying another boundary condition $y(l) = 0$ (to consider the other end of the beam):
\begin{gather}
  y(l) = -\frac{1}{EI}\left(-\frac{1}{2}M_Al^2-\frac{1}{24}wl^4+\frac{1}{6}R_Al^3\right) = 0 \\
  \longrightarrow \frac{1}{2}M_Al^2+\frac{1}{24}wl^4-\frac{1}{6}R_Al^3 = 0 \\
  \longrightarrow 12M_A + wl^2 - 4R_Al = 0
  \label{doubleintegration}
\end{gather}
The $R_A$, $R_B$, and $M_A$ are still \textbf{unknowns} at this point. Combining the equilibrium conditions with the double integration (equation (\ref{doubleintegration})):
\begin{gather}
  R_A-wl+R_B = 0 \\
  R_Al-M_A-\frac{1}{2}wl^2 = 0 \\
  4R_Al-12M_A-wl^2 = 0 
\end{gather}
Solving for the above system of equations yields:
\begin{gather}
  R_A = \frac{5}{8}wl \\
  R_B = \frac{3}{8}wl \\
  M_A = \frac{wl^2}{8}
\end{gather}
Using these values in all previous equations, all quantities can be determined.
\begin{figure}[H]
  \centering
  \includegraphics[width = 0.9 \textwidth]{../img/graph1.PNG}
\end{figure}
\subsubsection{Example: Fixed Beam with Concentrated Load (Macaulay's Method)}
\begin{figure}[H]
  \centering
  \includegraphics[width = 0.9 \textwidth]{../img/beam13.PNG}
\end{figure}
The equilibrium conditions:
\begin{gather}
  R_A-W+R_B = 0 \\
  M_A-Wb+R_AL-M_B = 0
\end{gather}
Moment at the point distance $x$ away from the left end:
\begin{gather}
  M(x) = M_A+R_Ax-W\langle x-a \rangle 
\end{gather}
Integrating the moment equation:
\begin{gather}
  \theta(x) = \frac{\dif y}{\dif x} = -\frac{1}{EI}\int\left(M_A+R_Ax-W\langle x-a \rangle\right) \dif x \\
  = -\frac{1}{EI}\left(M_Ax+\frac{1}{2}R_Ax^2-\frac{1}{2}W\langle x-a\rangle^2\right) + \theta_0
\end{gather}
Boundary Condition: $\theta(0) = 0 \longrightarrow \theta_0 = 0$
\begin{gather}
  \therefore \theta(x) = -\frac{1}{EI}\left(M_Ax+\frac{1}{2}R_Ax^2-\frac{1}{2}W\langle x-a\rangle^2\right)
\end{gather}
Integrating further:
\begin{gather}
  y(x) = -\frac{1}{EI}\int\left(M_Ax+\frac{1}{2}R_Ax^2-\frac{1}{2}W\langle x-a\rangle^2\right) \dif x \\
  = -\frac{1}{EI}\left(\frac{1}{2}M_Ax^2+\frac{1}{6}R_Ax^3-\frac{1}{6}W\langle x-a \rangle^3\right) + y_0
\end{gather}
Boundary Condition: $y(0) = 0 \longrightarrow y_0 = 0$
\begin{gather}
  \therefore y(x) = -\frac{1}{EI}\left(\frac{1}{2}M_Ax^2+\frac{1}{6}R_Ax^3-\frac{1}{6}W\langle x-a \rangle^3\right)
\end{gather}
Applying other boundary conditions $\theta(L) = 0$, $y(L) = 0$ (to consider the other end of the beam):
\begin{gather}
  \theta(L) = -\frac{1}{EI}\left(M_AL+\frac{1}{2}R_AL^2-\frac{1}{2}W(L-a)^2\right) = 0 \\
  y(L) = -\frac{1}{EI}\left(\frac{1}{2}M_AL^2+\frac{1}{6}R_AL^3-\frac{1}{6}W(L-a)^3\right) = 0
\end{gather}
\begin{gather}
  \text{Overall:}
  \begin{cases}
    R_A-W+R_B = 0 \\
    M_A-Wb+R_AL-M_B = 0 \\
    2M_AL+R_AL^2-W(L-a)^2 = 2M_AL+R_AL^2-Wb^2 = 0 \\
    3M_AL^2+R_AL^3-W(L-a)^3 = 3M_AL^2+R_AL^3-Wb^3 = 0
  \end{cases}
\end{gather}
The $R_A$, $R_B$, $M_A$, and $M_B$ are the 4 \textbf{unknowns} with 4 equations. Hence, they can be solved:
\begin{gather}
  R_A = \frac{Wb^2}{L^3}(3a+b) \\
  M_A = -\frac{Wab^2}{L^2} \\
  R_B = \frac{Wa^2}{L^3}(3b+a) \\
  M_B = -\frac{Wa^2b}{L^2}
\end{gather}
The equation of deflection:
\begin{gather}
  y = -\frac{W}{2EI}\left[\frac{b^2(3a+b)x^3}{3L^3}-\frac{ab^2x^2}{L^2}-\frac{\langle x-a \rangle^3}{3}\right] \\
  y(a) = \frac{Wa^3b^3}{3EIL^3}
\end{gather}
\begin{figure}[H]
  \centering
  \includegraphics[width = 0.9 \textwidth]{../img/graph2.PNG}
\end{figure}
\begin{figure}[H]
  \centering
  \includegraphics[width = 0.8 \textwidth]{../img/graph3.PNG}
  \caption{Depending on the loading, the profile of the deflection will be different. Maximum diflection occurs when $a=b=\frac{L}{2}$}
\end{figure}
Statically indeterminate structures produce \textbf{lower displacement and stress levels}, resulting in savings in material.
\textbf{Failure} of a member in a statically determinate structure \textbf{leads to collapse}. In case of failure of a member, statically indeterminate structures can find \textbf{alternative load paths}, at least temporarily.
\end{document}